feat: theorems upto flatten

octagon.v
@@ -194,25 +194,43 @@ Definition join(C C': list Constraint): list Constraint :=
     else cs
   ) C' C.
 
-Definition flatten(c: Constraint): list Constraint :=
-  match c with
-  | AddConstr l r d => 
-      if      l =? r      then [BndConstr l (d / 2)]
-      else if l =? (op r) then [] (* Delete these constraints *)
-      else [c]
-  | c => [c]
-  end.
+Definition normalize_constraint(c: Constraint): Constraint :=
+   match c with
+   | AddConstr l r d => 
+       if      l =? r      then BndConstr l (d / 2)
+       (* else if l =? - r then (1* Delete these constraints *1) *)
+       (* NOTE: While it would be useful to delete these constraints, since if it's satisifiable
+          then we can assume them to be of the sort 0 <= k for k natural, we don't include
+          a proof that the constraints are satisifiable, so for now it just complicates the
+          proof. It suffices that we normalize AddConstr t t d to BndConstr t (d/2) for now,
+          since this guarantees that flatten C = [] <-> C = [] *)
+       else c
+   | c => c
+   end.
+
+Definition flatten(C: list Constraint): list Constraint :=
+  map normalize_constraint C.
+
+Definition flatten_is_nil(C: list Constraint): flatten C = [] <-> C = [].
+Proof. (* {{{ *)
+  split; intros h; try (subst; reflexivity).
+  unfold flatten in h.
+  destruct C as [|c' C']; try reflexivity.
+  simpl in h.
+  unfold normalize_constraint in h.
+  destruct c'; [ destruct (l =? r) | idtac ]; discriminate.
+Qed. (* }}} *)
 
 Definition iterate(C: list Constraint) : list Constraint :=
   let C' := flat_map (fun c => flat_map (fun c' => opt_to_list(combine c c')) C) C in
-  let C'' := flat_map flatten C' in
+  let C'' := flatten C' in
   join C C''.
 
 Definition model : Type := nat -> Z.
 
 Definition term_value(m: model)(t: term): Z := proj1_sig t.(a) * (m t.(x)).
 
-Lemma term_value_op(m: model)(t: term): term_value m (-t) =  (- (term_value m t))%Z.
+Lemma term_value_op(t: term)(m: model): term_value m (-t) =  (- (term_value m t))%Z.
 Proof. (* {{{ *)
   unfold term_value.
   destruct t as [a x].
@@ -341,8 +359,17 @@ Proof. (* {{{ *)
   apply (Zplus_le_compat _ _ _ _ h h').
 Qed. (* }}} *)
 
+Lemma combine_mixed_constraints(x y z: Z)(d d': Z) :
+  x + y <= d
+  -> z <= d'
+  -> x + y + z <= d + d'.
+Proof. (* {{{ *)
+  intros h h'. 
+  apply (Zplus_le_compat _ _ _ _ h h').
+Qed. (* }}} *)
+
 Lemma nil_caract{A: Type}(ls: list A): (forall x, ~ In x ls) -> ls = [].
-Proof.
+Proof. (* {{{ *)
   intros no_mem_ls.
   destruct ls.
   - reflexivity.
@@ -351,7 +378,7 @@ Proof.
     apply no_mem_ls.
     Search (In ?x  (?x :: ?l)).
     apply in_eq.
-Qed.
+Qed. (* }}} *)
 
 Lemma superset_preserves_implication(C C': list Constraint)(c: Constraint) :
   (forall x, In x C -> In x C') ->
@@ -397,9 +424,71 @@ Proof. (* {{{ *)
     intros x. apply same_elems.
 Qed. (* }}} *)
 
+Lemma add_constr_are_commutable(l r: term)(d: Z) : 
+  (AddConstr l r d)  --> (AddConstr r l d).
+Proof. (* {{{ *)
+  intros m is_sat h.
+  subst is_sat.
+  simpl in *.
+  rewrite (Z.add_comm (term_value m r) (term_value m l)).
+  assumption.
+Qed. (* }}} *)
+
+(*
+| AddConstr l r d, AddConstr l' r' d' =>
+    if      l =? (op l') then Some (AddConstr r r' (d + d'))
+*)
+
+(* Lemma rule1(l r r': term)(d d': Z): *)
+(*   [AddConstr l r d; AddConstr (-r) r' d'] ==> AddConstr l r' (d + d'). *)
+(* Proof. *)
+(*   intros m. simpl. *)
+(*   Check term_value_op. *)
+(*   rewrite term_value_op. *)
+(*   intros h. apply Bool.andb_true_iff in h as [h h']. *)
+(*   rewrite Bool.andb_true_r in h'. *)
+(* Admitted. *)
+
+(* Ltac trial1 := *)
+(*   match goal with *)
+(*   | [ A : ?x + ?y <=? ?d |- _] => idtac *)
+(*   end. *)
+
+(* Ltac my_add_constr := *)
+(*   match goal with *)
+(*   | [ A : ?x + ?y <=? ?d |- _] *)
+(*   | [ A : ?y + ?x <=? ?d |- _] => *)
+(*       match goal with *)
+(*       | [ A' : -?x +  ?z <=? ?d' |- ] *)
+(*       | [ A' :  ?z + -?x <=? ?d' |- ] => *) 
+(*          match goal with *)
+(*            | [ |- ?y + ?z <=? (?d + ?d') ] *)
+(*            | [ |- ?z + ?y <=? (?d + ?d') ] => *) 
+(*                transitivity (- ?x + ?z + ?x + ?y); *) 
+(*                [ lia *) 
+(*                | apply (combine_addition_constraints _ _ _ _ _ _ A A') *)
+(*                ] *)
+(*          end *)
+(*       end *)
+(*   end. *)
+
+(*   | [ B : ?x <=? ?d *) 
+(*       |- ?z <=? (?d + ?d') *)
+(*       ] => *)
+(*       match goal with *)
+(*       | [ A' : - ?x + ?z <=? ?d' ] *)
+(*       | [ A' :   ?z + -?x <=? ?d' ] => *) 
+(*           transitivity (?x + - ?x + ?z); *)
+(*           [ lia *)
+(*           | apply ( *)
+(*           ] *)
+(*       | [ B' : ?y <=? ?d' ] => *)
+(*       end *)
+(*   end. *)
+
 Theorem combine_impl(c c' c'': Constraint) :
   combine c c' = Some c'' -> [c;c'] ==> c''.
-Proof.
+Proof. (* {{{ *)
   destruct c; destruct c' as [l' r' d' | t' d'].
   - unfold combine.
     destruct (l =?  - l') eqn:E.
@@ -410,7 +499,7 @@ Proof.
       intros m.
       simpl.
       Check term_value_op.
-      rewrite (term_value_op m _).
+      rewrite term_value_op.
       intros h.
       apply Bool.andb_true_iff in h as [h h'].
       Search (?x && true).
@@ -429,7 +518,7 @@ Proof.
       intros m.
       simpl.
       Check term_value_op.
-      rewrite (term_value_op m _).
+      rewrite term_value_op.
       intros h.
       apply Bool.andb_true_iff in h as [h h'].
       Search (?x && true).
@@ -441,14 +530,266 @@ Proof.
       transitivity (- term_value m r' + term_value m r + term_value m l' + term_value m r').
   ---- lia.
   ---- apply (combine_addition_constraints _ _ _ _ _ _ h h').
-  ---  (* TODO: Too much work for this demonstration *)
+  --- destruct E. destruct (r =? - l') eqn:E.
+  ---- intros h. injection h as h.
+       apply Term.eqb_eq in E.
+       subst c'' r.
+       intros m.
+       simpl.
+       Check term_value_op.
+       rewrite term_value_op.
+       intros h.
+       apply Bool.andb_true_iff in h as [h h'].
+       (* Search (?x && true). *)
+       rewrite -> (Bool.andb_true_r _) in h'.
 
-Admitted.
+       apply Zle_is_le_bool.
+       apply Zle_is_le_bool in h.
+       apply Zle_is_le_bool in h'.
+       transitivity (term_value m l + - term_value m l' + term_value m l' + term_value m r').
+       + lia.
+       + apply (combine_addition_constraints _ _ _ _ _ _ h h').
+  ---- destruct E. destruct (r =? - r') eqn:E.
+  ----- intros h. injection h as h.
+        apply Term.eqb_eq in E.
+        subst c'' r.
+        intros m.
+        simpl.
+        Check term_value_op.
+        rewrite term_value_op.
+        intros h.
+        apply Bool.andb_true_iff in h as [h h'].
+        (* Search (?x && true). *)
+        rewrite -> (Bool.andb_true_r _) in h'.
+
+        apply Zle_is_le_bool.
+        apply Zle_is_le_bool in h.
+        apply Zle_is_le_bool in h'.
+        transitivity (term_value m l + - term_value m r' + term_value m l' + term_value m r').
+        + lia.
+        + apply (combine_addition_constraints _ _ _ _ _ _ h h').
+  ----- discriminate.
+  - unfold combine.
+    destruct (l =? - t') eqn:E.
+  -- intros h. injection h as h.
+     apply Term.eqb_eq in E.
+     subst c'' l.
+     intros m.
+     simpl.
+     Check term_value_op.
+     rewrite term_value_op.
+     intros h.
+     apply Bool.andb_true_iff in h as [h h'].
+     (* Search (?x && true). *)
+     rewrite -> (Bool.andb_true_r _) in h'.
+
+     apply Zle_is_le_bool.
+     apply Zle_is_le_bool in h.
+     apply Zle_is_le_bool in h'.
+     transitivity (- term_value m t' + term_value m r + term_value m t').
+     + lia.
+     + apply (combine_mixed_constraints _ _ _ _ _ h h').
+  -- destruct E. destruct (r =? -t') eqn:E.
+  --- intros h. injection h as h.
+     apply Term.eqb_eq in E.
+     subst c'' r.
+     intros m.
+     simpl.
+     Check term_value_op.
+     rewrite term_value_op.
+     intros h.
+     apply Bool.andb_true_iff in h as [h h'].
+     (* Search (?x && true). *)
+     rewrite -> (Bool.andb_true_r _) in h'.
+
+     apply Zle_is_le_bool.
+     apply Zle_is_le_bool in h.
+     apply Zle_is_le_bool in h'.
+     transitivity (term_value m l + - term_value m t' + term_value m t').
+     + lia.
+     + apply (combine_mixed_constraints _ _ _ _ _ h h').
+  --- discriminate.
+  - unfold combine.
+    destruct (l' =? -t) eqn:E.
+  -- intros h. injection h as h.
+     apply Term.eqb_eq in E.
+     subst c'' l'.
+     intros m.
+     simpl.
+     Check term_value_op.
+     rewrite term_value_op.
+     intros h.
+     apply Bool.andb_true_iff in h as [h h'].
+     (* Search (?x && true). *)
+     rewrite -> (Bool.andb_true_r _) in h'.
+
+     apply Zle_is_le_bool.
+     apply Zle_is_le_bool in h.
+     apply Zle_is_le_bool in h'.
+     transitivity (- term_value m t + term_value m r' + term_value m t).
+     + lia.
+     + rewrite (Z.add_comm d).
+       apply (combine_mixed_constraints _ _ _ _ _ h' h).
+  -- destruct E. destruct (r' =? -t) eqn:E.
+  --- intros h. injection h as h.
+     apply Term.eqb_eq in E.
+     subst c'' r'.
+     intros m.
+     simpl.
+     Check term_value_op.
+     rewrite term_value_op.
+     intros h.
+     apply Bool.andb_true_iff in h as [h h'].
+     (* Search (?x && true). *)
+     rewrite -> (Bool.andb_true_r _) in h'.
+
+     apply Zle_is_le_bool.
+     apply Zle_is_le_bool in h.
+     apply Zle_is_le_bool in h'.
+     transitivity (term_value m l' + - term_value m t + term_value m t).
+     + lia.
+     + rewrite (Z.add_comm d).
+       apply (combine_mixed_constraints _ _ _ _ _ h' h).
+  --- discriminate.
+  - unfold combine.
+    intros h. injection h as h. subst.
+    intros m h.
+    apply Bool.andb_true_iff in h as [h h'].
+    (* Search (?x && true). *)
+    rewrite -> (Bool.andb_true_r _) in h'.
+
+    apply Zle_is_le_bool.
+    apply Zle_is_le_bool in h.
+    apply Zle_is_le_bool in h'.
+    apply (combine_bound_constraints _ _ _ _ h h').
+Qed.
+(* }}} *)
 
 Theorem impls_trans(C: list Constraint)(c c': Constraint) :
   (C ==> c) -> (c :: C ==> c') -> (C ==> c').
+Proof. (* {{{ *)
+  intros C_imp_c c_C_imp_c' m.
+  specialize (C_imp_c m).
+  specialize (c_C_imp_c' m).
+  destruct C eqn:E; try congruence.
+  rewrite <- E in *.
+  unfold satisfies_constraints.
+  intros h.
+  apply c_C_imp_c'.
+  unfold satisfies_constraints.
+  simpl.
+  apply Bool.andb_true_iff.
+  split; auto.
+Qed. (* }}} *)
+
+Print Z.
+Print positive.
+Search (nat -> Z).
+
+Lemma scale_monotonous(x y: Z)(k: nat): 
+  x <= y -> (Z.of_nat k * x <= Z.of_nat k*y).
+Proof. (* {{{ *)
+  induction k as [| k' IHk']; intros x_le_y.
+  - simpl. reflexivity.
+  - Search (Z.of_nat).
+    rewrite Nat2Z.inj_succ.
+    Search (Z.succ).
+    Check Z.mul_succ_l.
+    repeat rewrite Z.mul_succ_l.
+    Search (?x + ?y <= ?z + ?t).
+    Check Z.add_le_mono.
+    apply Z.add_le_mono; auto.
+Qed. (* }}} *)
+
+Theorem normalize_constraint_impl(c: Constraint):
+  forall m, satisfies_single_constraint m c = true <-> satisfies_single_constraint m (normalize_constraint c) = true.
+Proof with auto. (* {{{ *)
+  intros m.
+  unfold satisfies_single_constraint.
+  destruct c...
+  simpl. 
+  Search (?x <-> ?x).
+
+  destruct (l =? r) eqn:E.
+  - apply eqb_eq in E; subst.
+    split.
+  -- intros h; apply Zle_is_le_bool in h.
+     apply Zle_is_le_bool.
+     rewrite Z.add_diag in h.
+     Search (?x <= ?y -> ?x / ?k <= ?y / ?k).
+     apply (Z.div_le_mono _ _ 2) in h; try lia.
+     Search (?x * ?y = ?y * ?x).
+     rewrite (Z.mul_comm 2) in h.
+     Search (?x * ?k / ?k).
+     rewrite (Z.div_mul) in h; try (assumption || discriminate).
+  -- intros h; apply Zle_is_le_bool in h.
+     apply Zle_is_le_bool.
+     rewrite Z.add_diag.
+     Search (?x <= ?y -> ?k * ?x  <= ?k * ?y).
+     apply (Z.mul_le_mono_nonneg_l _ _ 2) in h; try lia.
+     apply Z.le_trans with (2*(d/2)); try lia.
+     apply Z.mul_div_le; try lia.
+  - simpl; apply iff_refl.
+  - simpl; apply iff_refl.
+Qed. (* }}} *)
+
+Lemma app_imp(C: list Constraint)(c c': Constraint):
+  (C ==> c') -> (c ::C ==> c').
+Proof. (* {{{ *)
+  intros C_imp_c' m.
+  specialize (C_imp_c' m).
+  destruct C as [|x xs]; try (exfalso; assumption).
+  intros h.
+  apply Bool.andb_true_iff in h as [h h'].
+  apply C_imp_c'.
+  unfold satisfies_constraints.
+  assumption.
+Qed. (* }}} *)
+
+Theorem flatten_impl(C: list Constraint)(c: Constraint) :
+  (C ==> c) -> (flatten C ==> c).
+Proof. (* {{{ *)
+  intros C_imp_c m.
+  specialize (C_imp_c m).
+  destruct C eqn:E; try (exfalso; assumption).
+  rewrite <- E in *.
+  destruct (flatten C) eqn:E'.
+  - rewrite E in E'. discriminate.
+  - rewrite <- E' in *.
+    intros h.
+    apply C_imp_c.
+    unfold flatten in h.
+    unfold satisfies_constraints in *.
+    apply forallb_forall.
+    rewrite forallb_forall in h.
+    intros x x_in_C.
+    Check in_map.
+    apply (in_map normalize_constraint) in x_in_C.
+    pose proof (h _ x_in_C) as h'.
+    apply normalize_constraint_impl; assumption.
+Qed. (* }}} *)
+
+(* NOTE: I should probably define the concept of "loses no information"
+         or "can be derived from" and reword the properties I want in
+         terms of these. So, if C =*=> C' means that with C I can derive
+         all of C', then we have to show that C =*=> (iterate C), which
+         is just showing the same thing for join, flatten and the nexted
+         flatmap with combine.
+         C =*=> C' can probably be forall c, In c C', (C ==> c)
+*)
+(* TODO: Rename flatten *)
+
+Theorem iterate_impl(C: list Constraint):
+  forall c, In c (iterate C) -> (C ==> c).
 Proof.
-Admitted.
+  intros c.
+  (* unfold iterate. *)
+
+Qed.
 
 End Octagon.
+
+
+
+
 
